seiostar/ExamplesIO.fst
@@ -6,9 +6,9 @@ let u_return () : io bool = return true
 
 let apply_io_return : bool -> io bool = fun x -> io_return x
 
-let apply_read () : io (resexn string) = read 0
-let apply_write_const () : io (resexn unit) = write (2,"hello")
-let apply_write : string -> io (resexn unit) = fun x -> write (1,x)
+let apply_read () : io (resexn string) = io_call ORead 0
+let apply_write_const () : io (resexn unit) = io_call OWrite (2,"hello")
+let apply_write : string -> io (resexn unit) = fun x -> io_call OWrite (1,x)
 
 let apply_io_bind_const () : io bool =
   let!@ x = io_return true in
@@ -26,20 +26,20 @@ let apply_io_bind_pure_if : bool -> io bool =
 
 let apply_io_bind_write : string -> io (resexn unit) =
   fun x ->
-    let!@ y = io_return x in
-    write (2,y)
+    let!@ y : string = io_return x in
+    io_call OWrite (2, y) <: io (resexn unit)
 
 let apply_io_bind_read_write () : io (resexn unit) =
-  match!@ read 4 with
-  | Inl _ -> write (1,"data")
+  match!@ io_call ORead 4 with
+  | Inl _ -> io_call OWrite (1,"data")
   | Inr x -> io_return (Inr x)
 
 let apply_io_bind_read_write' () : io (resexn unit) =
-  io_bind (read 9) (fun x -> match x with | Inl _ -> write (2,"data") | Inr x -> io_return (Inr x))
+  io_bind (io_call ORead 9) (fun x -> match x with | Inl _ -> io_call OWrite (2,"data") | Inr x -> io_return (Inr x))
 
 let apply_io_bind_read_if_write () : io (resexn unit) =
-  match!@ read 0 with
-  | Inl _ -> write (7,"data")
+  match!@ io_call ORead 0 with
+  | Inl _ -> io_call OWrite (7,"data")
   | Inr x -> return (Inr x)
 
 (** Examples inspired from the Web Server **)
@@ -47,12 +47,12 @@ val utf8_encode : bool -> bool
 let utf8_encode x = x
 
 let sendError400 (fd:bool) : io unit =
-  write (9, "error400") ;!@
+  io_call OWrite (9, "error400") ;!@
   return ()
 
 let get_req (fd:bool) : io (either bool bool) =
   let x = utf8_encode fd in
-  match!@ read 11 with
+  match!@ io_call ORead 11 with
   | Inl _ -> return (Inl true)
   | Inr _ -> return (Inr false)
 
@@ -62,15 +62,15 @@ let (let!@!) #a #b (m:io (resexn a)) (k:a -> io (resexn b)) =
   | Inr x -> io_return (Inr x)
 
 let open2_read_write () =
-  let!@! fd1 = openfile "/tmp/input" in
-  let!@! fd2 = openfile "/tmp/output" in
-  let!@! data = read fd1 in
-  write (fd2, data)
+  let!@! fd1 = io_call OOpen "/tmp/input" in
+  let!@! fd2 = io_call OOpen "/tmp/output" in
+  let!@! data = io_call ORead fd1 in
+  io_call OWrite (fd2, data)
 
 val eq_string : string -> string -> bool
 let eq_string s t =
   s = t
 
 let echo () =
-  let!@! data = read 0 in
-  write (1, data)
+  let!@! data = io_call ORead 0 in
+  io_call OWrite (1, data)
